crates/correctness/lean/MxxCorrectness/Generated/ToyExample/Ir.lean
@@ -12,7 +12,7 @@ def ToyExample_protocolSourceHash : String := "c894ed871c835c66f3dbb1c42a53b03a5
 
 def ToyExample_workflowHash : String := "f0727b300c312d49e01c5cba55cf8d11de69de7efa5d17b68a4133c5a6a15c6b"
 
-def ToyExample_toolkitHash : String := "6588c1ca3fd8b129c74321acc4446593704ed565d0791348883a4ffb684e84b8"
+def ToyExample_toolkitHash : String := "fe08e66d714d9275e61a20d1b9927610b3e31653f00da4283be711689ee2857a"
 
 def ToyExample_derivationHash : String := "1eb7ee1d85bf85dc59fea9e4e198e1cfa94df8fd0bf8168d408a754514520933"
 
